nasdaq/nordicequities/orderentry/NordicEquities_OrderEntry_v5_02_6_Server.lean
@@ -3025,7 +3025,7 @@ def encode (message : OrderAcceptedMessage) : List UInt8 :=
     ++ (encodeUInt 4 message.executionWithinFirm
     ++ (encodeUInt 4 message.investmentDecisionWithinFirmShortCode
     ++ (encodeUInt 4 message.clientIdentifier
-    ++ (encodeUIntLE 1 message.partyRoleQualifier
+    ++ (encodeUInt 1 message.partyRoleQualifier
     ++ (Capacity.encode message.capacity
     ++ (AlgoIndicator.encode message.algoIndicator
     ++ (encodeUInt 2 (BitVec.ofNat (8 * 2) (encodeMany Tagvalue.encode message.tagvalue.val).length)
@@ -3043,7 +3043,7 @@ def decode (bytes : List UInt8) : Option (OrderAcceptedMessage × List UInt8) :=
   let (executionWithinFirm, bytes) ← decodeUInt 4 bytes
   let (investmentDecisionWithinFirmShortCode, bytes) ← decodeUInt 4 bytes
   let (clientIdentifier, bytes) ← decodeUInt 4 bytes
-  let (partyRoleQualifier, bytes) ← decodeUIntLE 1 bytes
+  let (partyRoleQualifier, bytes) ← decodeUInt 1 bytes
   let (capacity, bytes) ← Capacity.decode bytes
   let (algoIndicator, bytes) ← AlgoIndicator.decode bytes
   let (appendageLength, bytes) ← decodeUInt 2 bytes
@@ -3061,7 +3061,7 @@ theorem encode_length_pos (message : OrderAcceptedMessage) : (encode message).le
 theorem encode_length_le (message : OrderAcceptedMessage) : (encode message).length ≤ 65591 := by
   have bound_tagvalue := message.tagvalue.length_lt
   unfold encode
-  simp only [List.length_append, ← Nat.add_assoc, encodeUInt_length, BuySellIndicator.encode_length, Alpha.encode_length, encodeUIntLE_length, Capacity.encode_length, AlgoIndicator.encode_length]
+  simp only [List.length_append, ← Nat.add_assoc, encodeUInt_length, BuySellIndicator.encode_length, Alpha.encode_length, Capacity.encode_length, AlgoIndicator.encode_length]
   omega
 
 @[simp] theorem decode_encode (message : OrderAcceptedMessage) (rest : List UInt8) :
@@ -3089,7 +3089,7 @@ theorem encode_length_le (message : OrderAcceptedMessage) : (encode message).len
   dsimp only
   rw [List.append_assoc, decodeUInt_encodeUInt, some_bind]
   dsimp only
-  rw [List.append_assoc, decodeUIntLE_encodeUIntLE, some_bind]
+  rw [List.append_assoc, decodeUInt_encodeUInt, some_bind]
   dsimp only
   rw [List.append_assoc, Capacity.decode_encode, some_bind]
   dsimp only
@@ -3350,7 +3350,7 @@ def encode (message : ExecutedOrderMessage) : List UInt8 :=
     ++ (TradingMode.encode message.tradingMode
     ++ (TransactionCategory.encode message.transactionCategory
     ++ (TransactionTypeAlgoIndicator.encode message.transactionTypeAlgoIndicator
-    ++ (encodeUIntLE 1 message.liquidityAttributes
+    ++ (encodeUInt 1 message.liquidityAttributes
     ++ (encodeUInt 1 message.lastMarket)))))))))))
 
 def decode (bytes : List UInt8) : Option (ExecutedOrderMessage × List UInt8) := do
@@ -3364,13 +3364,13 @@ def decode (bytes : List UInt8) : Option (ExecutedOrderMessage × List UInt8) :=
   let (tradingMode, bytes) ← TradingMode.decode bytes
   let (transactionCategory, bytes) ← TransactionCategory.decode bytes
   let (transactionTypeAlgoIndicator, bytes) ← TransactionTypeAlgoIndicator.decode bytes
-  let (liquidityAttributes, bytes) ← decodeUIntLE 1 bytes
+  let (liquidityAttributes, bytes) ← decodeUInt 1 bytes
   let (lastMarket, bytes) ← decodeUInt 1 bytes
   pure ({ timestamp, userRefNum, executedQuantity, executionPrice, liquidityFlag, matchNumber, contraFirm, tradingMode, transactionCategory, transactionTypeAlgoIndicator, liquidityAttributes, lastMarket }, bytes)
 
 @[simp] theorem encode_length (message : ExecutedOrderMessage) : (encode message).length = 34 := by
   unfold encode
-  simp only [List.length_append, encodeUInt_length, Alpha.encode_length, TradingMode.encode_length, TransactionCategory.encode_length, TransactionTypeAlgoIndicator.encode_length, encodeUIntLE_length]
+  simp only [List.length_append, encodeUInt_length, Alpha.encode_length, TradingMode.encode_length, TransactionCategory.encode_length, TransactionTypeAlgoIndicator.encode_length]
 
 theorem encode_length_pos (message : ExecutedOrderMessage) : (encode message).length > 0 := by
   rw [encode_length]
@@ -3399,7 +3399,7 @@ theorem encode_length_pos (message : ExecutedOrderMessage) : (encode message).le
   dsimp only
   rw [List.append_assoc, TransactionTypeAlgoIndicator.decode_encode, some_bind]
   dsimp only
-  rw [List.append_assoc, decodeUIntLE_encodeUIntLE, some_bind]
+  rw [List.append_assoc, decodeUInt_encodeUInt, some_bind]
   dsimp only
   rw [decodeUInt_encodeUInt, some_bind]
   rfl
